IMLTT/typed/proofs/Recursor.lean
@@ -77,15 +77,12 @@ theorem judgment_recursor :
     (a_1 : Γ ⊢ f ∶ (.pi A B)) (a_2 : Γ ⊢ a ∶ A),
     motive_3 Γ f (.pi A B) a_1 → motive_3 Γ a A a_2 
     → motive_3 Γ (.app f a) (substitute_zero a B) (HasType.pi_elim a_1 a_2))
-  → (HasTypeSigmaElim : ∀ {n : Nat} {Γ : Ctx n} {A : Tm n} {B : Tm (n + 1)} {p : Tm n} 
-    {C : Tm (n + 1)} {c : Tm (n + 1 + 1)}
-    (a_1 : Γ ⊢ p ∶ (.sigma A B)) (a_2 : (Γ ⬝ (.sigma A B)) ⊢ C type)
-    (a_3 : (Γ ⬝ A ⬝ B) ⊢ c ∶ (substitute (Subst.weak (.shift (.shift .id)), 
-      (.pairSigma v(1) v(0))) C)),
-    motive_3 Γ p (.sigma A B) a_1 → motive_2 (Γ ⬝ (.sigma A B)) C a_2
-    → motive_3 (Γ ⬝ A ⬝ B) c
-      (substitute (Subst.weak (.shift (.shift .id)), (.pairSigma v(1) v(0))) C) a_3
-    → motive_3 Γ (.indSigma A B C c p) (substitute_zero p C) (HasType.sigma_elim a_1 a_2 a_3) )
+  → (HasTypeSigmaFirst : ∀ {n : Nat} {Γ : Ctx n} {p A : Tm n} {B : Tm (n + 1)}
+    (a_1 : Γ ⊢ p ∶ (ΣA;B)), motive_3 Γ p (ΣA;B) a_1
+    → motive_3 Γ (π₁ p) A (HasType.sigma_first a_1))
+  → (HasTypeSigmaSecond : ∀ {n : Nat} {Γ : Ctx n} {p A : Tm n} {B : Tm (n + 1)}
+    (a_1 : Γ ⊢ p ∶ (ΣA;B)), motive_3 Γ p (ΣA;B) a_1
+    → motive_3 Γ (π₂ p) (B⌈π₁ p⌉₀) (HasType.sigma_second a_1))
   → (HasTypeIdenElim : ∀ {n : Nat} {Γ : Ctx n} {A : Tm n} {B : Tm (n + 1 + 1 + 1)} {b : Tm n} 
     {a a' p : Tm n}
     (a_1 : (Γ ⬝ A ⬝ (weaken Weak.id.shift A) ⬝ (weaken Weak.id.shift.shift A).iden v(1) v(0)) ⊢ B type)
@@ -145,15 +142,15 @@ theorem judgment_recursor :
     (a_1 : (Γ ⬝ A) ⊢ b ∶ B) (a_2 : Γ ⊢ a ∶ A), motive_3 (Γ ⬝ A) b B a_1 → motive_3 Γ a A a_2 
     → motive_5 Γ ((A.lam b).app a) (substitute_zero a b) (substitute_zero a B) 
       (IsEqualTerm.pi_comp a_1 a_2))
-  → (IsEqualTermSigmaComp : ∀ {n : Nat} {Γ : Ctx n} {a A b : Tm n} {B C : Tm (n + 1)} 
-    {c : Tm (n + 1 + 1)} (a_1 : Γ ⊢ a ∶ A)
-    (a_2 : Γ ⊢ b ∶ substitute_zero a B) (a_3 : (Γ ⬝ A.sigma B) ⊢ C type)
-    (a_4 : (Γ ⬝ A ⬝ B) ⊢ c ∶ substitute (Subst.weak Weak.id.shift.shift, v(1).pairSigma v(0)) C),
-    motive_3 Γ a A a_1 → motive_3 Γ b (substitute_zero a B) a_2 → motive_2 (Γ ⬝ A.sigma B) C a_3 
-    → motive_3 (Γ ⬝ A ⬝ B) c (substitute (Subst.weak Weak.id.shift.shift, v(1).pairSigma v(0)) C) a_4 
-    → motive_5 Γ (A.indSigma B C c (a.pairSigma b)) (substitute (Subst.weak Weak.id, a, b) c)
-      (substitute_zero (a.pairSigma b) C) (IsEqualTerm.sigma_comp a_1 a_2 a_3 a_4))
-  → (IsEqualTermIdenComp : ∀ {n : Nat} {Γ : Ctx n} {A : Tm n} {B : Tm (n + 1 + 1 + 1)} 
+  → (IsEqualTermSigmaFirstComp : ∀ {n : Nat} {Γ : Ctx n} {a b A : Tm n} {B : Tm (n + 1)}
+    (a_1 : Γ ⊢ a ∶ A) (a_2 : Γ ⊢ b ∶ B⌈a⌉₀) (a_3 : Γ ⊢ (ΣA;B) type), 
+    motive_3 Γ a A a_1 → motive_3 Γ b (B⌈a⌉₀) a_2 → motive_2 Γ (ΣA;B) a_3
+    → motive_5 Γ (π₁ (.pairSigma a b)) a A (IsEqualTerm.sigma_first_comp a_1 a_2 a_3))
+  → (IsEqualTermSigmaSecondComp : ∀ {n : Nat} {Γ : Ctx n} {a b A : Tm n} {B : Tm (n + 1)}
+    (a_1 : Γ ⊢ a ∶ A) (a_2 : Γ ⊢ b ∶ B⌈a⌉₀) (a_3 : Γ ⊢ (ΣA;B) type), 
+    motive_3 Γ a A a_1 → motive_3 Γ b (B⌈a⌉₀) a_2 → motive_2 Γ (ΣA;B) a_3
+    → motive_5 Γ (π₂ (.pairSigma a b)) b (B⌈π₁ a&b⌉₀) (IsEqualTerm.sigma_second_comp a_1 a_2 a_3))
+  → (IsEqualTermIdenComp : ∀ {n : Nat} {Γ : Ctx n} {A : Tm n} {B : Tm (n + 1 + 1 + 1)}
     {b : Tm n} {a : Tm n}
     (a_1 : (Γ ⬝ A ⬝ (weaken Weak.id.shift A) ⬝ (weaken Weak.id.shift.shift A).iden v(1) v(0)) ⊢ B type)
     (a_2 : Γ ⊢ b ∶ (substitute (Subst.weak Weak.id, a, a, .refl A a) B))
@@ -187,16 +184,12 @@ theorem judgment_recursor :
     (a_1 : Γ ⊢ a ≡ a' ∶ A) (a_2 : Γ ⊢ b ≡ b' ∶ substitute_zero a B) (a_3 : Γ ⬝ A ⊢ B type),
     motive_5 Γ a a' A a_1 → motive_5 Γ b b' (substitute_zero a B) a_2 → motive_2 (Γ ⬝ A) (B) a_3
     → motive_5 Γ (a.pairSigma b) (a'.pairSigma b') (A.sigma B) (IsEqualTerm.sigma_intro_eq a_1 a_2 a_3))
-  → (IsEqualTermSigmaElimEq :  ∀ {n : Nat} {Γ : Ctx n} {A : Tm n} {B : Tm (n + 1)} {A' : Tm n} 
-    {B' : Tm (n + 1)} {p p' : Tm n} {C C' : Tm (n + 1)} {c c' : Tm (n + 1 + 1)} 
-    (a : Γ ⊢ A ≡ A' type) (a_4 : (Γ ⬝ A) ⊢ B ≡ B' type) (a_1 : Γ ⊢ p ≡ p' ∶ A.sigma B)
-    (a_2 : (Γ ⬝ A.sigma B) ⊢ C ≡ C' type)
-    (a_3 : (Γ ⬝ A ⬝ B) ⊢ c ≡ c' ∶ substitute (Subst.weak Weak.id.shift.shift, v(1).pairSigma v(0)) C),
-    motive_4 Γ A A' a → motive_4 (Γ ⬝ A) B B' a_4 → motive_5 Γ p p' (A.sigma B) a_1 
-    → motive_4 (Γ ⬝ A.sigma B) C C' a_2
-    → motive_5 (Γ ⬝ A ⬝ B) c c' (substitute (Subst.weak Weak.id.shift.shift, v(1).pairSigma v(0)) C) a_3
-    → motive_5 Γ (A.indSigma B C c p) (A'.indSigma B' C' c' p') (substitute_zero p C)
-      (IsEqualTerm.sigma_elim_eq a a_4 a_1 a_2 a_3))
+  → (IsEqualTermSigmaFirstEq : ∀ {n : Nat} {Γ : Ctx n} {p p' A : Tm n} {B : Tm (n + 1)}
+    (a_1 : Γ ⊢ p ≡ p' ∶ (ΣA;B)), motive_5 Γ p p' (ΣA;B) a_1
+    → motive_5 Γ (π₁ p) (π₁ p') A (IsEqualTerm.sigma_first_eq a_1))
+  → (IsEqualTermSigmaSecondEq : ∀ {n : Nat} {Γ : Ctx n} {p p' A : Tm n} {B : Tm (n + 1)}
+    (a_1 : Γ ⊢ p ≡ p' ∶ (ΣA;B)), motive_5 Γ p p' (ΣA;B) a_1
+    → motive_5 Γ (π₂ p) (π₂ p') (B⌈π₁ p⌉₀) (IsEqualTerm.sigma_second_eq a_1))
   → (IsEqualTermIdenIntroEq : ∀ {n : Nat} {Γ : Ctx n} {A A' a a' : Tm n} 
     (a_1 : Γ ⊢ A ≡ A' type) (a_2 : Γ ⊢ a ≡ a' ∶ A), motive_4 Γ A A' a_1 → motive_5 Γ a a' A a_2 
     → motive_5 Γ (A.refl a) (A'.refl a') (A.iden a a) (IsEqualTerm.iden_intro_eq a_1 a_2))
@@ -256,14 +249,16 @@ theorem judgment_recursor :
           hIsTypeUnivForm hIsTypeUnivElim
     intro hHasTypeVar hHasTypeWeak hHasTypeUnitIntro hHasTypePiIntro hHasTypeSigmaIntro hHasTypeIdenIntro
           hHasTypeUnivUnit hHasTypeUnivEmpty hHasTypeUnivPi hHasTypeUnivSigma hHasTypeUnivIden
-          hHasTypeUnitElim hHasTypeEmptyElim hHasTypePiElim hHasTypeSigmaElim hHasTypeIdenElim
+          hHasTypeUnitElim hHasTypeEmptyElim hHasTypePiElim hHasTypeSigmaFirst hHasTypeSigmaSecond hHasTypeIdenElim
           hHasTypeTyConv
     intro hIsEqualTypeUnitFormEq hIsEqualTypeEmptyFormEQ hIsEqualTypePiFormEq hIsEqualTypeSigmaFormEq
           hIsEqualTypeIdenFormEq hIsEqalTypeUnivFormEq hIsEqualTypeUnivElimEq
           hIsEqualTypeTypeSymm hIsEqualTypeTypeTrans
-    intro hIsEqualTermVarEq hIsEqualTermWeakEq hIsEqualTermUnitComp hIsEqualTermPiComp hIsEqualTermSigmaComp
+    intro hIsEqualTermVarEq hIsEqualTermWeakEq hIsEqualTermUnitComp hIsEqualTermPiComp
+          hIsEqualTermSigmaFirstComp hIsEqualTermSigmaSecondComp
           hIsEqualTermIdenComp hIsEqualTermUnitIntroEq hIsEqualTermUnitElimEq hIsEqualTermEmptyElimEq
-          hIsEqualTermPiIntroEq hIsEqualTermPiElimEq hIsEqualTermSigmaIntroEq hIsEqualTermSigmaElimEq
+          hIsEqualTermPiIntroEq hIsEqualTermPiElimEq hIsEqualTermSigmaIntroEq
+          hIsEqualTermSigmaFirstEq hIsEqualTermSigmaSecondEq
           hIsEqualTermIdenIntroEq hIsEqualTermIdenElimEq hIsEqualTermUnivUnitEq
           hIsEqualTermUnivEmptyEq hIsEqualTermUnivPiEq hIsEqualTermUnivSigmaEq
           hIsEqualTermUnivIdenEq hIsEqualTermTyConvEq
@@ -279,14 +274,16 @@ theorem judgment_recursor :
           hIsTypeUnivForm hIsTypeUnivElim
         hHasTypeVar hHasTypeWeak hHasTypeUnitIntro hHasTypePiIntro hHasTypeSigmaIntro hHasTypeIdenIntro
           hHasTypeUnivUnit hHasTypeUnivEmpty hHasTypeUnivPi hHasTypeUnivSigma hHasTypeUnivIden
-          hHasTypeUnitElim hHasTypeEmptyElim hHasTypePiElim hHasTypeSigmaElim hHasTypeIdenElim
+          hHasTypeUnitElim hHasTypeEmptyElim hHasTypePiElim hHasTypeSigmaFirst hHasTypeSigmaSecond hHasTypeIdenElim
           hHasTypeTyConv
         hIsEqualTypeUnitFormEq hIsEqualTypeEmptyFormEQ hIsEqualTypePiFormEq hIsEqualTypeSigmaFormEq
           hIsEqualTypeIdenFormEq hIsEqalTypeUnivFormEq hIsEqualTypeUnivElimEq
           hIsEqualTypeTypeSymm hIsEqualTypeTypeTrans
-        hIsEqualTermVarEq hIsEqualTermWeakEq hIsEqualTermUnitComp hIsEqualTermPiComp hIsEqualTermSigmaComp
+        hIsEqualTermVarEq hIsEqualTermWeakEq hIsEqualTermUnitComp hIsEqualTermPiComp 
+          hIsEqualTermSigmaFirstComp hIsEqualTermSigmaSecondComp
           hIsEqualTermIdenComp hIsEqualTermUnitIntroEq hIsEqualTermUnitElimEq hIsEqualTermEmptyElimEq
-          hIsEqualTermPiIntroEq hIsEqualTermPiElimEq hIsEqualTermSigmaIntroEq hIsEqualTermSigmaElimEq
+          hIsEqualTermPiIntroEq hIsEqualTermPiElimEq hIsEqualTermSigmaIntroEq
+          hIsEqualTermSigmaFirstEq hIsEqualTermSigmaSecondEq
           hIsEqualTermIdenIntroEq hIsEqualTermIdenElimEq hIsEqualTermUnivUnitEq 
           hIsEqualTermUnivEmptyEq hIsEqualTermUnivPiEq hIsEqualTermUnivSigmaEq 
           hIsEqualTermUnivIdenEq hIsEqualTermTyConvEq
@@ -301,14 +298,16 @@ theorem judgment_recursor :
           hIsTypeUnivForm hIsTypeUnivElim
         hHasTypeVar hHasTypeWeak hHasTypeUnitIntro hHasTypePiIntro hHasTypeSigmaIntro hHasTypeIdenIntro
           hHasTypeUnivUnit hHasTypeUnivEmpty hHasTypeUnivPi hHasTypeUnivSigma hHasTypeUnivIden
-          hHasTypeUnitElim hHasTypeEmptyElim hHasTypePiElim hHasTypeSigmaElim hHasTypeIdenElim
+          hHasTypeUnitElim hHasTypeEmptyElim hHasTypePiElim hHasTypeSigmaFirst hHasTypeSigmaSecond hHasTypeIdenElim
           hHasTypeTyConv
         hIsEqualTypeUnitFormEq hIsEqualTypeEmptyFormEQ hIsEqualTypePiFormEq hIsEqualTypeSigmaFormEq
           hIsEqualTypeIdenFormEq hIsEqalTypeUnivFormEq hIsEqualTypeUnivElimEq
           hIsEqualTypeTypeSymm hIsEqualTypeTypeTrans
-        hIsEqualTermVarEq hIsEqualTermWeakEq hIsEqualTermUnitComp hIsEqualTermPiComp hIsEqualTermSigmaComp
+        hIsEqualTermVarEq hIsEqualTermWeakEq hIsEqualTermUnitComp hIsEqualTermPiComp 
+          hIsEqualTermSigmaFirstComp hIsEqualTermSigmaSecondComp
           hIsEqualTermIdenComp hIsEqualTermUnitIntroEq hIsEqualTermUnitElimEq hIsEqualTermEmptyElimEq
-          hIsEqualTermPiIntroEq hIsEqualTermPiElimEq hIsEqualTermSigmaIntroEq hIsEqualTermSigmaElimEq
+          hIsEqualTermPiIntroEq hIsEqualTermPiElimEq hIsEqualTermSigmaIntroEq
+          hIsEqualTermSigmaFirstEq hIsEqualTermSigmaSecondEq
           hIsEqualTermIdenIntroEq hIsEqualTermIdenElimEq hIsEqualTermUnivUnitEq 
           hIsEqualTermUnivEmptyEq hIsEqualTermUnivPiEq hIsEqualTermUnivSigmaEq 
           hIsEqualTermUnivIdenEq hIsEqualTermTyConvEq
@@ -323,14 +322,16 @@ theorem judgment_recursor :
           hIsTypeUnivForm hIsTypeUnivElim
         hHasTypeVar hHasTypeWeak hHasTypeUnitIntro hHasTypePiIntro hHasTypeSigmaIntro hHasTypeIdenIntro
           hHasTypeUnivUnit hHasTypeUnivEmpty hHasTypeUnivPi hHasTypeUnivSigma hHasTypeUnivIden
-          hHasTypeUnitElim hHasTypeEmptyElim hHasTypePiElim hHasTypeSigmaElim hHasTypeIdenElim
+          hHasTypeUnitElim hHasTypeEmptyElim hHasTypePiElim hHasTypeSigmaFirst hHasTypeSigmaSecond hHasTypeIdenElim
           hHasTypeTyConv
         hIsEqualTypeUnitFormEq hIsEqualTypeEmptyFormEQ hIsEqualTypePiFormEq hIsEqualTypeSigmaFormEq
           hIsEqualTypeIdenFormEq hIsEqalTypeUnivFormEq hIsEqualTypeUnivElimEq
           hIsEqualTypeTypeSymm hIsEqualTypeTypeTrans
-        hIsEqualTermVarEq hIsEqualTermWeakEq hIsEqualTermUnitComp hIsEqualTermPiComp hIsEqualTermSigmaComp
+        hIsEqualTermVarEq hIsEqualTermWeakEq hIsEqualTermUnitComp hIsEqualTermPiComp 
+          hIsEqualTermSigmaFirstComp hIsEqualTermSigmaSecondComp
           hIsEqualTermIdenComp hIsEqualTermUnitIntroEq hIsEqualTermUnitElimEq hIsEqualTermEmptyElimEq
-          hIsEqualTermPiIntroEq hIsEqualTermPiElimEq hIsEqualTermSigmaIntroEq hIsEqualTermSigmaElimEq
+          hIsEqualTermPiIntroEq hIsEqualTermPiElimEq hIsEqualTermSigmaIntroEq
+          hIsEqualTermSigmaFirstEq hIsEqualTermSigmaSecondEq
           hIsEqualTermIdenIntroEq hIsEqualTermIdenElimEq hIsEqualTermUnivUnitEq 
           hIsEqualTermUnivEmptyEq hIsEqualTermUnivPiEq hIsEqualTermUnivSigmaEq 
           hIsEqualTermUnivIdenEq hIsEqualTermTyConvEq
@@ -345,14 +346,16 @@ theorem judgment_recursor :
           hIsTypeUnivForm hIsTypeUnivElim
         hHasTypeVar hHasTypeWeak hHasTypeUnitIntro hHasTypePiIntro hHasTypeSigmaIntro hHasTypeIdenIntro
           hHasTypeUnivUnit hHasTypeUnivEmpty hHasTypeUnivPi hHasTypeUnivSigma hHasTypeUnivIden
-          hHasTypeUnitElim hHasTypeEmptyElim hHasTypePiElim hHasTypeSigmaElim hHasTypeIdenElim
+          hHasTypeUnitElim hHasTypeEmptyElim hHasTypePiElim hHasTypeSigmaFirst hHasTypeSigmaSecond hHasTypeIdenElim
           hHasTypeTyConv
         hIsEqualTypeUnitFormEq hIsEqualTypeEmptyFormEQ hIsEqualTypePiFormEq hIsEqualTypeSigmaFormEq
           hIsEqualTypeIdenFormEq hIsEqalTypeUnivFormEq hIsEqualTypeUnivElimEq
           hIsEqualTypeTypeSymm hIsEqualTypeTypeTrans
-        hIsEqualTermVarEq hIsEqualTermWeakEq hIsEqualTermUnitComp hIsEqualTermPiComp hIsEqualTermSigmaComp
+        hIsEqualTermVarEq hIsEqualTermWeakEq hIsEqualTermUnitComp hIsEqualTermPiComp 
+          hIsEqualTermSigmaFirstComp hIsEqualTermSigmaSecondComp
           hIsEqualTermIdenComp hIsEqualTermUnitIntroEq hIsEqualTermUnitElimEq hIsEqualTermEmptyElimEq
-          hIsEqualTermPiIntroEq hIsEqualTermPiElimEq hIsEqualTermSigmaIntroEq hIsEqualTermSigmaElimEq
+          hIsEqualTermPiIntroEq hIsEqualTermPiElimEq hIsEqualTermSigmaIntroEq
+          hIsEqualTermSigmaFirstEq hIsEqualTermSigmaSecondEq
           hIsEqualTermIdenIntroEq hIsEqualTermIdenElimEq hIsEqualTermUnivUnitEq 
           hIsEqualTermUnivEmptyEq hIsEqualTermUnivPiEq hIsEqualTermUnivSigmaEq 
           hIsEqualTermUnivIdenEq hIsEqualTermTyConvEq
@@ -367,14 +370,16 @@ theorem judgment_recursor :
           hIsTypeUnivForm hIsTypeUnivElim
         hHasTypeVar hHasTypeWeak hHasTypeUnitIntro hHasTypePiIntro hHasTypeSigmaIntro hHasTypeIdenIntro
           hHasTypeUnivUnit hHasTypeUnivEmpty hHasTypeUnivPi hHasTypeUnivSigma hHasTypeUnivIden
-          hHasTypeUnitElim hHasTypeEmptyElim hHasTypePiElim hHasTypeSigmaElim hHasTypeIdenElim
+          hHasTypeUnitElim hHasTypeEmptyElim hHasTypePiElim hHasTypeSigmaFirst hHasTypeSigmaSecond hHasTypeIdenElim
           hHasTypeTyConv
         hIsEqualTypeUnitFormEq hIsEqualTypeEmptyFormEQ hIsEqualTypePiFormEq hIsEqualTypeSigmaFormEq
           hIsEqualTypeIdenFormEq hIsEqalTypeUnivFormEq hIsEqualTypeUnivElimEq
           hIsEqualTypeTypeSymm hIsEqualTypeTypeTrans
-        hIsEqualTermVarEq hIsEqualTermWeakEq hIsEqualTermUnitComp hIsEqualTermPiComp hIsEqualTermSigmaComp
+        hIsEqualTermVarEq hIsEqualTermWeakEq hIsEqualTermUnitComp hIsEqualTermPiComp 
+          hIsEqualTermSigmaFirstComp hIsEqualTermSigmaSecondComp
           hIsEqualTermIdenComp hIsEqualTermUnitIntroEq hIsEqualTermUnitElimEq hIsEqualTermEmptyElimEq
-          hIsEqualTermPiIntroEq hIsEqualTermPiElimEq hIsEqualTermSigmaIntroEq hIsEqualTermSigmaElimEq
+          hIsEqualTermPiIntroEq hIsEqualTermPiElimEq hIsEqualTermSigmaIntroEq
+          hIsEqualTermSigmaFirstEq hIsEqualTermSigmaSecondEq
           hIsEqualTermIdenIntroEq hIsEqualTermIdenElimEq hIsEqualTermUnivUnitEq 
           hIsEqualTermUnivEmptyEq hIsEqualTermUnivPiEq hIsEqualTermUnivSigmaEq 
           hIsEqualTermUnivIdenEq hIsEqualTermTyConvEq
