IMLTT/typed/proofs/admissable/FunctionalityTyping/HasType.lean
@@ -1199,71 +1199,37 @@ theorem functionality_typing_pi_elim :
         · apply hsS'
         repeat' rfl
 
-theorem functionality_typing_sigma_elim :
-  ∀ {n : Nat} {Γ : Ctx n} {A : Tm n} {B : Tm (n + 1)} {p : Tm n} {C : Tm (n + 1)} {c : Tm (n + 1 + 1)},
-  (Γ ⊢ p ∶ ΣA;B) →
-   (Γ ⬝ ΣA;B) ⊢ C type →
-     (Γ ⬝ A ⬝ B ⊢ c ∶ C⌈(ₛ↑ₚ↑ₚidₚ), v(1)&v(0)⌉) →
-       ((∀ (m l k : Nat) {leq : l ≤ m} (Γ_1 : Ctx l) (Δ : CtxGen (l + 1) (m + 1)) (Ξ : CtxGen (m + 2) (k + 1))
-             (eqM : n = k + 1) (s s' S : Tm l) (T : Tm (m + 1)),
-             (Γ_1 ⊢ s ≡ s' ∶ S) →
-               (Γ_1 ⊢ s ∶ S) →
-                 (Γ_1 ⊢ s' ∶ S) →
-                   eqM ▸ Γ = Γ_1 ⬝ S ⊗ Δ ⊙ T ⊗ Ξ → Γ_1 ⊗ ⌈s⌉(Δ w/Nat.le_refl l) ⊢ T⌈s/ₙleq⌉ ≡ T⌈s'/ₙleq⌉ type) ∧
-           ∀ (m l : Nat) {leq : l ≤ m} (Γ_1 : Ctx l) (Δ : CtxGen (l + 1) (m + 1)) (s s' S : Tm l) (t T : Tm (m + 1))
-             (eqM : n = m + 1),
-             (Γ_1 ⊢ s ≡ s' ∶ S) →
-               (Γ_1 ⊢ s ∶ S) →
-                 (Γ_1 ⊢ s' ∶ S) →
-                   eqM ▸ Γ = Γ_1 ⬝ S ⊗ Δ →
-                     eqM ▸ p = t →
-                       (eqM ▸ ΣA;B) = T → Γ_1 ⊗ ⌈s⌉(Δ w/Nat.le_refl l) ⊢ t⌈s/ₙleq⌉ ≡ t⌈s'/ₙleq⌉ ∶ T⌈s/ₙleq⌉) →
-         ((∀ (m l k : Nat) {leq : l ≤ m} (Γ_1 : Ctx l) (Δ : CtxGen (l + 1) (m + 1)) (Ξ : CtxGen (m + 2) (k + 1))
-               (eqM : n + 1 = k + 1) (s s' S : Tm l) (T : Tm (m + 1)),
-               (Γ_1 ⊢ s ≡ s' ∶ S) →
-                 (Γ_1 ⊢ s ∶ S) →
-                   (Γ_1 ⊢ s' ∶ S) →
-                     (eqM ▸ Γ ⬝ ΣA;B) = Γ_1 ⬝ S ⊗ Δ ⊙ T ⊗ Ξ →
-                       Γ_1 ⊗ ⌈s⌉(Δ w/Nat.le_refl l) ⊢ T⌈s/ₙleq⌉ ≡ T⌈s'/ₙleq⌉ type) ∧
-             ∀ (m l : Nat) {leq : l ≤ m} (Γ_1 : Ctx l) (Δ : CtxGen (l + 1) (m + 1)) (s s' S : Tm l) (T : Tm (m + 1))
-               (eqM : n + 1 = m + 1),
-               (Γ_1 ⊢ s ≡ s' ∶ S) →
-                 (Γ_1 ⊢ s ∶ S) →
-                   (Γ_1 ⊢ s' ∶ S) →
-                     (eqM ▸ Γ ⬝ ΣA;B) = Γ_1 ⬝ S ⊗ Δ →
-                       eqM ▸ C = T → Γ_1 ⊗ ⌈s⌉(Δ w/Nat.le_refl l) ⊢ T⌈s/ₙleq⌉ ≡ T⌈s'/ₙleq⌉ type) →
-           ((∀ (m l k : Nat) {leq : l ≤ m} (Γ_1 : Ctx l) (Δ : CtxGen (l + 1) (m + 1)) (Ξ : CtxGen (m + 2) (k + 1))
-                 (eqM : n + 1 + 1 = k + 1) (s s' S : Tm l) (T : Tm (m + 1)),
-                 (Γ_1 ⊢ s ≡ s' ∶ S) →
-                   (Γ_1 ⊢ s ∶ S) →
-                     (Γ_1 ⊢ s' ∶ S) →
-                       eqM ▸ Γ ⬝ A ⬝ B = Γ_1 ⬝ S ⊗ Δ ⊙ T ⊗ Ξ →
-                         Γ_1 ⊗ ⌈s⌉(Δ w/Nat.le_refl l) ⊢ T⌈s/ₙleq⌉ ≡ T⌈s'/ₙleq⌉ type) ∧
-               ∀ (m l : Nat) {leq : l ≤ m} (Γ_1 : Ctx l) (Δ : CtxGen (l + 1) (m + 1)) (s s' S : Tm l)
-                 (t T : Tm (m + 1)) (eqM : n + 1 + 1 = m + 1),
-                 (Γ_1 ⊢ s ≡ s' ∶ S) →
-                   (Γ_1 ⊢ s ∶ S) →
-                     (Γ_1 ⊢ s' ∶ S) →
-                       eqM ▸ Γ ⬝ A ⬝ B = Γ_1 ⬝ S ⊗ Δ →
-                         eqM ▸ c = t →
-                           eqM ▸ C⌈(ₛ↑ₚ↑ₚidₚ), v(1)&v(0)⌉ = T →
-                             Γ_1 ⊗ ⌈s⌉(Δ w/Nat.le_refl l) ⊢ t⌈s/ₙleq⌉ ≡ t⌈s'/ₙleq⌉ ∶ T⌈s/ₙleq⌉) →
-             (∀ (m l k : Nat) {leq : l ≤ m} (Γ_1 : Ctx l) (Δ : CtxGen (l + 1) (m + 1)) (Ξ : CtxGen (m + 2) (k + 1))
-                 (eqM : n = k + 1) (s s' S : Tm l) (T : Tm (m + 1)),
-                 (Γ_1 ⊢ s ≡ s' ∶ S) →
-                   (Γ_1 ⊢ s ∶ S) →
-                     (Γ_1 ⊢ s' ∶ S) →
-                       eqM ▸ Γ = Γ_1 ⬝ S ⊗ Δ ⊙ T ⊗ Ξ → Γ_1 ⊗ ⌈s⌉(Δ w/Nat.le_refl l) ⊢ T⌈s/ₙleq⌉ ≡ T⌈s'/ₙleq⌉ type) ∧
-               ∀ (m l : Nat) {leq : l ≤ m} (Γ_1 : Ctx l) (Δ : CtxGen (l + 1) (m + 1)) (s s' S : Tm l)
-                 (t T : Tm (m + 1)) (eqM : n = m + 1),
-                 (Γ_1 ⊢ s ≡ s' ∶ S) →
-                   (Γ_1 ⊢ s ∶ S) →
-                     (Γ_1 ⊢ s' ∶ S) →
-                       eqM ▸ Γ = Γ_1 ⬝ S ⊗ Δ →
-                         eqM ▸ A.indSigma B C c p = t →
-                           eqM ▸ C⌈p⌉₀ = T → Γ_1 ⊗ ⌈s⌉(Δ w/Nat.le_refl l) ⊢ t⌈s/ₙleq⌉ ≡ t⌈s'/ₙleq⌉ ∶ T⌈s/ₙleq⌉ :=
+theorem functionality_typing_sigma_first :
+    ∀ {n : Nat} {Γ : Ctx n} {p A : Tm n} {B : Tm (n + 1)},
+    (Γ ⊢ p ∶ ΣA;B) →
+    ((∀ (m l k : Nat) {leq : l ≤ m} (Γ_1 : Ctx l) (Δ : CtxGen (l + 1) (m + 1)) (Ξ : CtxGen (m + 2) (k + 1))
+          (eqM : n = k + 1) (s s' S : Tm l) (T : Tm (m + 1)),
+          (Γ_1 ⊢ s ≡ s' ∶ S) →
+            (Γ_1 ⊢ s ∶ S) →
+              (Γ_1 ⊢ s' ∶ S) →
+                eqM ▸ Γ = Γ_1 ⬝ S ⊗ Δ ⊙ T ⊗ Ξ → Γ_1 ⊗ ⌈s⌉(Δ w/Nat.le_refl l) ⊢ T⌈s/ₙleq⌉ ≡ T⌈s'/ₙleq⌉ type) ∧
+        ∀ (m l : Nat) {leq : l ≤ m} (Γ_1 : Ctx l) (Δ : CtxGen (l + 1) (m + 1)) (s s' S : Tm l) (t T : Tm (m + 1))
+          (eqM : n = m + 1),
+          (Γ_1 ⊢ s ≡ s' ∶ S) →
+            (Γ_1 ⊢ s ∶ S) →
+              (Γ_1 ⊢ s' ∶ S) →
+                eqM ▸ Γ = Γ_1 ⬝ S ⊗ Δ →
+                  eqM ▸ p = t → (eqM ▸ ΣA;B) = T → Γ_1 ⊗ ⌈s⌉(Δ w/Nat.le_refl l) ⊢ t⌈s/ₙleq⌉ ≡ t⌈s'/ₙleq⌉ ∶ T⌈s/ₙleq⌉) →
+      (∀ (m l k : Nat) {leq : l ≤ m} (Γ_1 : Ctx l) (Δ : CtxGen (l + 1) (m + 1)) (Ξ : CtxGen (m + 2) (k + 1))
+          (eqM : n = k + 1) (s s' S : Tm l) (T : Tm (m + 1)),
+          (Γ_1 ⊢ s ≡ s' ∶ S) →
+            (Γ_1 ⊢ s ∶ S) →
+              (Γ_1 ⊢ s' ∶ S) →
+                eqM ▸ Γ = Γ_1 ⬝ S ⊗ Δ ⊙ T ⊗ Ξ → Γ_1 ⊗ ⌈s⌉(Δ w/Nat.le_refl l) ⊢ T⌈s/ₙleq⌉ ≡ T⌈s'/ₙleq⌉ type) ∧
+        ∀ (m l : Nat) {leq : l ≤ m} (Γ_1 : Ctx l) (Δ : CtxGen (l + 1) (m + 1)) (s s' S : Tm l) (t T : Tm (m + 1))
+          (eqM : n = m + 1),
+          (Γ_1 ⊢ s ≡ s' ∶ S) →
+            (Γ_1 ⊢ s ∶ S) →
+              (Γ_1 ⊢ s' ∶ S) →
+                eqM ▸ Γ = Γ_1 ⬝ S ⊗ Δ →
+                  eqM ▸ π₁ p = t → eqM ▸ A = T → Γ_1 ⊗ ⌈s⌉(Δ w/Nat.le_refl l) ⊢ t⌈s/ₙleq⌉ ≡ t⌈s'/ₙleq⌉ ∶ T⌈s/ₙleq⌉ :=
   by
-    intro n Γ' A B p C c hpSi hC hcC ihpSi ihC ihcC
+    intro n Γ' p A B hpSi ihpSi
     apply And.intro
     · intro m l k hleq Γ Δ Ξ heqM s s' S T hssS hsS hsS' heqΓ
       cases heqM
@@ -1282,29 +1248,10 @@ theorem functionality_typing_sigma_elim :
       cases heqΓ
       cases heqt
       cases heqT
-      simp [substitution_zero_lift]
-      apply IsEqualTerm.sigma_elim_eq
-      · apply And.left ihcC
-        · apply hssS
-        · apply hsS
-        · apply hsS'
-        rotate_left
-        · apply m + 1 + 1
-        · apply CtxGen.start ⊙ B
-        · rfl
-        · rfl
-      · simp [lift_subst_n]
-        simp [lift_n_substitution]
-        rw [extend_expand_context_n_substitution]
-        apply And.left ihcC
-        · apply hssS
-        · apply hsS
-        · apply hsS'
-        rotate_left
-        · apply m + 1 + 1
-        · apply CtxGen.start
-        · rfl
-        · rfl
+      simp []
+      apply IsEqualTerm.sigma_first_eq
+      rotate_left
+      · apply B⌈1ₙ⇑ₛ(s/ₙhleq)⌉
       · simp [lift_subst_n]
         rw [←substitution_sigma]
         apply And.right ihpSi
@@ -1312,26 +1259,39 @@ theorem functionality_typing_sigma_elim :
         · apply hsS
         · apply hsS'
         repeat' rfl
-      · simp [lift_subst_n]
-        rw [←substitution_sigma]
-        rw [lift_n_substitution]
-        rw [lift_n_substitution]
-        rw [extend_expand_context_n_substitution]
-        apply And.right ihC
-        · apply hssS
-        · apply hsS
-        · apply hsS'
-        repeat' rfl
-      · simp [lift_subst_n]
-        rw [subst_subst_sigma_C]
-        simp [lift_n_substitution]
-        rw [extend_expand_context_n_substitution]
-        rw [extend_expand_context_n_substitution]
-        apply And.right ihcC
-        · apply hssS
-        · apply hsS
-        · apply hsS'
-        repeat' rfl
+
+theorem functionality_typing_sigma_second :
+    ∀ {n : Nat} {Γ : Ctx n} {p A : Tm n} {B : Tm (n + 1)},
+    (Γ ⊢ p ∶ ΣA;B) →
+    ((∀ (m l k : Nat) {leq : l ≤ m} (Γ_1 : Ctx l) (Δ : CtxGen (l + 1) (m + 1)) (Ξ : CtxGen (m + 2) (k + 1))
+          (eqM : n = k + 1) (s s' S : Tm l) (T : Tm (m + 1)),
+          (Γ_1 ⊢ s ≡ s' ∶ S) →
+            (Γ_1 ⊢ s ∶ S) →
+              (Γ_1 ⊢ s' ∶ S) →
+                eqM ▸ Γ = Γ_1 ⬝ S ⊗ Δ ⊙ T ⊗ Ξ → Γ_1 ⊗ ⌈s⌉(Δ w/Nat.le_refl l) ⊢ T⌈s/ₙleq⌉ ≡ T⌈s'/ₙleq⌉ type) ∧
+        ∀ (m l : Nat) {leq : l ≤ m} (Γ_1 : Ctx l) (Δ : CtxGen (l + 1) (m + 1)) (s s' S : Tm l) (t T : Tm (m + 1))
+          (eqM : n = m + 1),
+          (Γ_1 ⊢ s ≡ s' ∶ S) →
+            (Γ_1 ⊢ s ∶ S) →
+              (Γ_1 ⊢ s' ∶ S) →
+                eqM ▸ Γ = Γ_1 ⬝ S ⊗ Δ →
+                  eqM ▸ p = t → (eqM ▸ ΣA;B) = T → Γ_1 ⊗ ⌈s⌉(Δ w/Nat.le_refl l) ⊢ t⌈s/ₙleq⌉ ≡ t⌈s'/ₙleq⌉ ∶ T⌈s/ₙleq⌉) →
+      (∀ (m l k : Nat) {leq : l ≤ m} (Γ_1 : Ctx l) (Δ : CtxGen (l + 1) (m + 1)) (Ξ : CtxGen (m + 2) (k + 1))
+          (eqM : n = k + 1) (s s' S : Tm l) (T : Tm (m + 1)),
+          (Γ_1 ⊢ s ≡ s' ∶ S) →
+            (Γ_1 ⊢ s ∶ S) →
+              (Γ_1 ⊢ s' ∶ S) →
+                eqM ▸ Γ = Γ_1 ⬝ S ⊗ Δ ⊙ T ⊗ Ξ → Γ_1 ⊗ ⌈s⌉(Δ w/Nat.le_refl l) ⊢ T⌈s/ₙleq⌉ ≡ T⌈s'/ₙleq⌉ type) ∧
+        ∀ (m l : Nat) {leq : l ≤ m} (Γ_1 : Ctx l) (Δ : CtxGen (l + 1) (m + 1)) (s s' S : Tm l) (t T : Tm (m + 1))
+          (eqM : n = m + 1),
+          (Γ_1 ⊢ s ≡ s' ∶ S) →
+            (Γ_1 ⊢ s ∶ S) →
+              (Γ_1 ⊢ s' ∶ S) →
+                eqM ▸ Γ = Γ_1 ⬝ S ⊗ Δ →
+                  eqM ▸ π₂ p = t →
+                    eqM ▸ B⌈π₁ p⌉₀ = T → Γ_1 ⊗ ⌈s⌉(Δ w/Nat.le_refl l) ⊢ t⌈s/ₙleq⌉ ≡ t⌈s'/ₙleq⌉ ∶ T⌈s/ₙleq⌉ :=
+  by
+    sorry
 
 theorem functionality_typing_iden_elim :
   ∀ {n : Nat} {Γ : Ctx n} {A : Tm n} {B : Tm (n + 1 + 1 + 1)} {b a a' p : Tm n},
