IMLTT/typed/proofs/admissable/Substitution/IsEqualTerm.lean
@@ -258,82 +258,104 @@ theorem substitution_gen_pi_comp : ∀ {n : Nat} {Γ : Ctx n} {A : Tm n} {b B : 
       · apply hsS
       · rfl
 
-theorem substitution_gen_sigma_comp : ∀ {n : Nat} {Γ : Ctx n} {a A b : Tm n} {B C : Tm (n + 1)} {c : Tm (n + 1 + 1)},
-   (Γ ⊢ a ∶ A) →
-     (Γ ⊢ b ∶ B⌈a⌉₀) →
-       (Γ ⬝ ΣA;B) ⊢ C type →
-         (Γ ⬝ A ⬝ B ⊢ c ∶ C⌈(ₛ↑ₚ↑ₚidₚ), v(1)&v(0)⌉) →
-           (∀ (m l : Nat) {leq : l ≤ m} (Γ_1 : Ctx l) (Δ : CtxGen (l + 1) (m + 1)) (eqM : n = m + 1) (s S : Tm l)
-               (a_5 A_1 : Tm (m + 1 - 1 + 1)),
-               eqM ▸ Γ = Γ_1 ⬝ S ⊗ Δ →
-                 eqM ▸ a = a_5 →
-                   eqM ▸ A = A_1 → (Γ_1 ⊢ s ∶ S) → Γ_1 ⊗ ⌈s⌉(Δ w/Nat.le_refl l) ⊢ a_5⌈s/ₙleq⌉ ∶ A_1⌈s/ₙleq⌉) →
-             (∀ (m l : Nat) {leq : l ≤ m} (Γ_1 : Ctx l) (Δ : CtxGen (l + 1) (m + 1)) (eqM : n = m + 1) (s S : Tm l)
-                 (a_6 A : Tm (m + 1 - 1 + 1)),
-                 eqM ▸ Γ = Γ_1 ⬝ S ⊗ Δ →
-                   eqM ▸ b = a_6 →
-                     eqM ▸ B⌈a⌉₀ = A → (Γ_1 ⊢ s ∶ S) → Γ_1 ⊗ ⌈s⌉(Δ w/Nat.le_refl l) ⊢ a_6⌈s/ₙleq⌉ ∶ A⌈s/ₙleq⌉) →
-               (∀ (m l : Nat) {leq : l ≤ m} (Γ_1 : Ctx l) (Δ : CtxGen (l + 1) (m + 1)) (eqM : n + 1 = m + 1) {s S : Tm l}
-                   (A_1 : Tm (m + 1 - 1 + 1)),
-                   (eqM ▸ Γ ⬝ ΣA;B) = Γ_1 ⬝ S ⊗ Δ →
-                     eqM ▸ C = A_1 → (Γ_1 ⊢ s ∶ S) → Γ_1 ⊗ ⌈s⌉(Δ w/Nat.le_refl l) ⊢ A_1⌈s/ₙleq⌉ type) →
-                 (∀ (m l : Nat) {leq : l ≤ m} (Γ_1 : Ctx l) (Δ : CtxGen (l + 1) (m + 1)) (eqM : n + 1 + 1 = m + 1)
-                     (s S : Tm l) (a A_1 : Tm (m + 1 - 1 + 1)),
-                     eqM ▸ Γ ⬝ A ⬝ B = Γ_1 ⬝ S ⊗ Δ →
-                       eqM ▸ c = a →
-                         eqM ▸ C⌈(ₛ↑ₚ↑ₚidₚ), v(1)&v(0)⌉ = A_1 →
-                           (Γ_1 ⊢ s ∶ S) → Γ_1 ⊗ ⌈s⌉(Δ w/Nat.le_refl l) ⊢ a⌈s/ₙleq⌉ ∶ A_1⌈s/ₙleq⌉) →
-                   ∀ (m l : Nat) {leq : l ≤ m} (Γ_1 : Ctx l) (Δ : CtxGen (l + 1) (m + 1)) (eqM : n = m + 1) (s S : Tm l)
-                     (a_9 a' A_1 : Tm (m + 1 - 1 + 1)),
-                     eqM ▸ Γ = Γ_1 ⬝ S ⊗ Δ →
-                       eqM ▸ A.indSigma B C c (a&b) = a_9 →
-                         eqM ▸ c⌈(ₛidₚ), a, b⌉ = a' →
-                           eqM ▸ C⌈a&b⌉₀ = A_1 →
-                             (Γ_1 ⊢ s ∶ S) → Γ_1 ⊗ ⌈s⌉(Δ w/Nat.le_refl l) ⊢ a_9⌈s/ₙleq⌉ ≡ a'⌈s/ₙleq⌉ ∶ A_1⌈s/ₙleq⌉ :=
+theorem substitution_gen_sigma_first_comp :
+    ∀ {n : Nat} {Γ : Ctx n} {a b A : Tm n} {B : Tm (n + 1)},
+    (Γ ⊢ a ∶ A) →
+    (Γ ⊢ b ∶ B⌈a⌉₀) →
+      Γ ⊢ ΣA;B type →
+        (∀ (m l : Nat) {leq : l ≤ m} (Γ_1 : Ctx l) (Δ : CtxGen (l + 1) (m + 1)) (eqM : n = m + 1) (s S : Tm l)
+            (a_4 A_1 : Tm (m + 1 - 1 + 1)),
+            eqM ▸ Γ = Γ_1 ⬝ S ⊗ Δ →
+              eqM ▸ a = a_4 →
+                eqM ▸ A = A_1 → (Γ_1 ⊢ s ∶ S) → Γ_1 ⊗ ⌈s⌉(Δ w/Nat.le_refl l) ⊢ a_4⌈s/ₙleq⌉ ∶ A_1⌈s/ₙleq⌉) →
+          (∀ (m l : Nat) {leq : l ≤ m} (Γ_1 : Ctx l) (Δ : CtxGen (l + 1) (m + 1)) (eqM : n = m + 1) (s S : Tm l)
+              (a_5 A : Tm (m + 1 - 1 + 1)),
+              eqM ▸ Γ = Γ_1 ⬝ S ⊗ Δ →
+                eqM ▸ b = a_5 →
+                  eqM ▸ B⌈a⌉₀ = A → (Γ_1 ⊢ s ∶ S) → Γ_1 ⊗ ⌈s⌉(Δ w/Nat.le_refl l) ⊢ a_5⌈s/ₙleq⌉ ∶ A⌈s/ₙleq⌉) →
+            (∀ (m l : Nat) {leq : l ≤ m} (Γ_1 : Ctx l) (Δ : CtxGen (l + 1) (m + 1)) (eqM : n = m + 1) {s S : Tm l}
+                (A_1 : Tm (m + 1 - 1 + 1)),
+                eqM ▸ Γ = Γ_1 ⬝ S ⊗ Δ →
+                  (eqM ▸ ΣA;B) = A_1 → (Γ_1 ⊢ s ∶ S) → Γ_1 ⊗ ⌈s⌉(Δ w/Nat.le_refl l) ⊢ A_1⌈s/ₙleq⌉ type) →
+              ∀ (m l : Nat) {leq : l ≤ m} (Γ_1 : Ctx l) (Δ : CtxGen (l + 1) (m + 1)) (eqM : n = m + 1) (s S : Tm l)
+                (a_7 a' A_1 : Tm (m + 1 - 1 + 1)),
+                eqM ▸ Γ = Γ_1 ⬝ S ⊗ Δ →
+                  eqM ▸ π₁ a&b = a_7 →
+                    eqM ▸ a = a' →
+                      eqM ▸ A = A_1 →
+                        (Γ_1 ⊢ s ∶ S) → Γ_1 ⊗ ⌈s⌉(Δ w/Nat.le_refl l) ⊢ a_7⌈s/ₙleq⌉ ≡ a'⌈s/ₙleq⌉ ∶ A_1⌈s/ₙleq⌉ :=
   by
-    intro n Γ' a A b B C c haA hbB hC hcC ihaA ihbB ihC ihcC m l hleq Γ Δ heqM s S t t' T heqΓ heqt heqt' heqT hsS
+    intro n Γ' a b A B haA hbB hSi ihaA ihbB ihSi m l hleq Γ Δ heqM s S t t' T heqΓ heqt heqt' heqT hsS
+    cases heqM
+    cases heqΓ
+    cases heqt
+    cases heqt'
+    cases heqT
+    apply IsEqualTerm.sigma_first_comp
+    rotate_right
+    · apply B⌈1ₙ⇑ₛ(s/ₙhleq)⌉
+    · apply ihaA
+      repeat' rfl
+      apply hsS
+    · simp [lift_subst_n]
+      simp [←substitution_zero_lift]
+      apply ihbB
+      repeat' rfl
+      apply hsS
+    · simp [lift_subst_n]
+      rw [←substitution_sigma]
+      apply ihSi
+      repeat' rfl
+      apply hsS
+
+theorem substitution_gen_sigma_second_comp :
+    ∀ {n : Nat} {Γ : Ctx n} {a b A : Tm n} {B : Tm (n + 1)},
+    (Γ ⊢ a ∶ A) →
+    (Γ ⊢ b ∶ B⌈a⌉₀) →
+      Γ ⊢ ΣA;B type →
+        (∀ (m l : Nat) {leq : l ≤ m} (Γ_1 : Ctx l) (Δ : CtxGen (l + 1) (m + 1)) (eqM : n = m + 1) (s S : Tm l)
+            (a_4 A_1 : Tm (m + 1 - 1 + 1)),
+            eqM ▸ Γ = Γ_1 ⬝ S ⊗ Δ →
+              eqM ▸ a = a_4 →
+                eqM ▸ A = A_1 → (Γ_1 ⊢ s ∶ S) → Γ_1 ⊗ ⌈s⌉(Δ w/Nat.le_refl l) ⊢ a_4⌈s/ₙleq⌉ ∶ A_1⌈s/ₙleq⌉) →
+          (∀ (m l : Nat) {leq : l ≤ m} (Γ_1 : Ctx l) (Δ : CtxGen (l + 1) (m + 1)) (eqM : n = m + 1) (s S : Tm l)
+              (a_5 A : Tm (m + 1 - 1 + 1)),
+              eqM ▸ Γ = Γ_1 ⬝ S ⊗ Δ →
+                eqM ▸ b = a_5 →
+                  eqM ▸ B⌈a⌉₀ = A → (Γ_1 ⊢ s ∶ S) → Γ_1 ⊗ ⌈s⌉(Δ w/Nat.le_refl l) ⊢ a_5⌈s/ₙleq⌉ ∶ A⌈s/ₙleq⌉) →
+            (∀ (m l : Nat) {leq : l ≤ m} (Γ_1 : Ctx l) (Δ : CtxGen (l + 1) (m + 1)) (eqM : n = m + 1) {s S : Tm l}
+                (A_1 : Tm (m + 1 - 1 + 1)),
+                eqM ▸ Γ = Γ_1 ⬝ S ⊗ Δ →
+                  (eqM ▸ ΣA;B) = A_1 → (Γ_1 ⊢ s ∶ S) → Γ_1 ⊗ ⌈s⌉(Δ w/Nat.le_refl l) ⊢ A_1⌈s/ₙleq⌉ type) →
+              ∀ (m l : Nat) {leq : l ≤ m} (Γ_1 : Ctx l) (Δ : CtxGen (l + 1) (m + 1)) (eqM : n = m + 1) (s S : Tm l)
+                (a_7 a' A : Tm (m + 1 - 1 + 1)),
+                eqM ▸ Γ = Γ_1 ⬝ S ⊗ Δ →
+                  eqM ▸ π₂ a&b = a_7 →
+                    eqM ▸ b = a' →
+                      eqM ▸ B⌈π₁ a&b⌉₀ = A →
+                        (Γ_1 ⊢ s ∶ S) → Γ_1 ⊗ ⌈s⌉(Δ w/Nat.le_refl l) ⊢ a_7⌈s/ₙleq⌉ ≡ a'⌈s/ₙleq⌉ ∶ A⌈s/ₙleq⌉ :=
+  by
+    intro n Γ' a b A B haA hbB hSi ihaA ihbB ihSi m l hleq Γ Δ heqM s S t t' T heqΓ heqt heqt' heqT hsS
     cases heqM
     cases heqΓ
     cases heqt
     cases heqt'
     cases heqT
     simp [substitution_zero_lift]
-    rw [subst_subst_sigma_c]
-    apply IsEqualTerm.sigma_comp
+    apply IsEqualTerm.sigma_second_comp
+    rotate_right
+    · apply A⌈(s/ₙhleq)⌉
     · apply ihaA
-      · rfl
-      · rfl
-      · rfl
-      · apply hsS
-      · rfl
-    · simp [lift_subst_n]
-      simp [←substitution_zero_lift]
+      repeat' rfl
+      apply hsS
+    · simp [←substitution_zero_lift]
       apply ihbB
-      · rfl
-      · rfl
-      · rfl
-      · apply hsS
-      · rfl
-    · simp [lift_subst_n]
-      rw [←substitution_sigma]
-      rw [lift_n_substitution]
-      rw [extend_expand_context_n_substitution]
-      apply ihC
-      · rfl
-      · rfl
-      · apply hsS
-      · rfl
-    · simp [lift_subst_n]
-      rw [subst_subst_sigma_C]
-      simp [lift_n_substitution]
-      rw [extend_expand_context_n_substitution]
-      rw [extend_expand_context_n_substitution]
-      apply ihcC
-      · rfl
-      · rfl
-      · rfl
-      · apply hsS
-      · rfl
+      repeat' rfl
+      apply hsS
+    · rw [←substitution_sigma]
+      apply ihSi
+      repeat' rfl
+      apply hsS
 
 theorem substitution_gen_iden_comp : ∀ {n : Nat} {Γ : Ctx n} {A : Tm n} {B : Tm (n + 1 + 1 + 1)} {b a : Tm n},
    (Γ ⬝ A ⬝ A⌊↑ₚidₚ⌋ ⬝ v(1) ≃[A⌊↑ₚ↑ₚidₚ⌋] v(0)) ⊢ B type →
@@ -734,105 +756,69 @@ theorem substitution_gen_sigma_intro_eq :
       · apply hsS
       · rfl
 
-theorem substitution_gen_sigma_elim_eq : ∀ {n : Nat} {Γ : Ctx n} {A : Tm n} {B : Tm (n + 1)} {A' : Tm n} {B' : Tm (n + 1)} {p p' : Tm n} {C C' : Tm (n + 1)}
-    {c c' : Tm (n + 1 + 1)},
-    Γ ⊢ A ≡ A' type →
-      Γ ⬝ A ⊢ B ≡ B' type →
-        (Γ ⊢ p ≡ p' ∶ ΣA;B) →
-          (Γ ⬝ ΣA;B) ⊢ C ≡ C' type →
-            (Γ ⬝ A ⬝ B ⊢ c ≡ c' ∶ C⌈(ₛ↑ₚ↑ₚidₚ), v(1)&v(0)⌉) →
-              (∀ (m l : Nat) {leq : l ≤ m} (Γ_1 : Ctx l) (Δ : CtxGen (l + 1) (m + 1)) (eqM : n = m + 1) (s S : Tm l)
-                  (A_1 A'_1 : Tm (m + 1 - 1 + 1)),
-                  eqM ▸ Γ = Γ_1 ⬝ S ⊗ Δ →
-                    eqM ▸ A = A_1 →
-                      eqM ▸ A' = A'_1 → (Γ_1 ⊢ s ∶ S) → Γ_1 ⊗ ⌈s⌉(Δ w/Nat.le_refl l) ⊢ A_1⌈s/ₙleq⌉ ≡ A'_1⌈s/ₙleq⌉ type) →
-                (∀ (m l : Nat) {leq : l ≤ m} (Γ_1 : Ctx l) (Δ : CtxGen (l + 1) (m + 1)) (eqM : n + 1 = m + 1) (s S : Tm l)
-                    (A_1 A' : Tm (m + 1 - 1 + 1)),
-                    eqM ▸ Γ ⬝ A = Γ_1 ⬝ S ⊗ Δ →
-                      eqM ▸ B = A_1 →
-                        eqM ▸ B' = A' → (Γ_1 ⊢ s ∶ S) → Γ_1 ⊗ ⌈s⌉(Δ w/Nat.le_refl l) ⊢ A_1⌈s/ₙleq⌉ ≡ A'⌈s/ₙleq⌉ type) →
-                  (∀ (m l : Nat) {leq : l ≤ m} (Γ_1 : Ctx l) (Δ : CtxGen (l + 1) (m + 1)) (eqM : n = m + 1) (s S : Tm l)
-                      (a a' A_1 : Tm (m + 1 - 1 + 1)),
-                      eqM ▸ Γ = Γ_1 ⬝ S ⊗ Δ →
-                        eqM ▸ p = a →
-                          eqM ▸ p' = a' →
-                            (eqM ▸ ΣA;B) = A_1 →
-                              (Γ_1 ⊢ s ∶ S) → Γ_1 ⊗ ⌈s⌉(Δ w/Nat.le_refl l) ⊢ a⌈s/ₙleq⌉ ≡ a'⌈s/ₙleq⌉ ∶ A_1⌈s/ₙleq⌉) →
-                    (∀ (m l : Nat) {leq : l ≤ m} (Γ_1 : Ctx l) (Δ : CtxGen (l + 1) (m + 1)) (eqM : n + 1 = m + 1)
-                        (s S : Tm l) (A_1 A' : Tm (m + 1 - 1 + 1)),
-                        (eqM ▸ Γ ⬝ ΣA;B) = Γ_1 ⬝ S ⊗ Δ →
-                          eqM ▸ C = A_1 →
-                            eqM ▸ C' = A' →
-                              (Γ_1 ⊢ s ∶ S) → Γ_1 ⊗ ⌈s⌉(Δ w/Nat.le_refl l) ⊢ A_1⌈s/ₙleq⌉ ≡ A'⌈s/ₙleq⌉ type) →
-                      (∀ (m l : Nat) {leq : l ≤ m} (Γ_1 : Ctx l) (Δ : CtxGen (l + 1) (m + 1)) (eqM : n + 1 + 1 = m + 1)
-                          (s S : Tm l) (a a' A_1 : Tm (m + 1 - 1 + 1)),
-                          eqM ▸ Γ ⬝ A ⬝ B = Γ_1 ⬝ S ⊗ Δ →
-                            eqM ▸ c = a →
-                              eqM ▸ c' = a' →
-                                eqM ▸ C⌈(ₛ↑ₚ↑ₚidₚ), v(1)&v(0)⌉ = A_1 →
-                                  (Γ_1 ⊢ s ∶ S) → Γ_1 ⊗ ⌈s⌉(Δ w/Nat.le_refl l) ⊢ a⌈s/ₙleq⌉ ≡ a'⌈s/ₙleq⌉ ∶ A_1⌈s/ₙleq⌉) →
-                        ∀ (m l : Nat) {leq : l ≤ m} (Γ_1 : Ctx l) (Δ : CtxGen (l + 1) (m + 1)) (eqM : n = m + 1)
-                          (s S : Tm l) (a a' A_1 : Tm (m + 1 - 1 + 1)),
-                          eqM ▸ Γ = Γ_1 ⬝ S ⊗ Δ →
-                            eqM ▸ A.indSigma B C c p = a →
-                              eqM ▸ A'.indSigma B' C' c' p' = a' →
-                                eqM ▸ C⌈p⌉₀ = A_1 →
-                                  (Γ_1 ⊢ s ∶ S) → Γ_1 ⊗ ⌈s⌉(Δ w/Nat.le_refl l) ⊢ a⌈s/ₙleq⌉ ≡ a'⌈s/ₙleq⌉ ∶ A_1⌈s/ₙleq⌉ :=
+theorem substitution_gen_sigma_first_eq :
+    ∀ {n : Nat} {Γ : Ctx n} {p p' A : Tm n} {B : Tm (n + 1)},
+    (Γ ⊢ p ≡ p' ∶ ΣA;B) →
+    (∀ (m l : Nat) {leq : l ≤ m} (Γ_1 : Ctx l) (Δ : CtxGen (l + 1) (m + 1)) (eqM : n = m + 1) (s S : Tm l)
+        (a a' A_1 : Tm (m + 1 - 1 + 1)),
+        eqM ▸ Γ = Γ_1 ⬝ S ⊗ Δ →
+          eqM ▸ p = a →
+            eqM ▸ p' = a' →
+              (eqM ▸ ΣA;B) = A_1 →
+                (Γ_1 ⊢ s ∶ S) → Γ_1 ⊗ ⌈s⌉(Δ w/Nat.le_refl l) ⊢ a⌈s/ₙleq⌉ ≡ a'⌈s/ₙleq⌉ ∶ A_1⌈s/ₙleq⌉) →
+      ∀ (m l : Nat) {leq : l ≤ m} (Γ_1 : Ctx l) (Δ : CtxGen (l + 1) (m + 1)) (eqM : n = m + 1) (s S : Tm l)
+        (a a' A_1 : Tm (m + 1 - 1 + 1)),
+        eqM ▸ Γ = Γ_1 ⬝ S ⊗ Δ →
+          eqM ▸ π₁ p = a →
+            eqM ▸ π₁ p' = a' →
+              eqM ▸ A = A_1 → (Γ_1 ⊢ s ∶ S) → Γ_1 ⊗ ⌈s⌉(Δ w/Nat.le_refl l) ⊢ a⌈s/ₙleq⌉ ≡ a'⌈s/ₙleq⌉ ∶ A_1⌈s/ₙleq⌉ :=
   by
-    intro n Γ' A B A' B' p p' C C' c c' hAA hBB hppSi hCC hccC ihAA ihBB ihppSi ihCC ihccC m l hleq Γ Δ heqM s S t t' T heqΓ heqt heqt' heqT hsS
+    intro n Γ' p p' A B hppSi ihppSi m l hleq Γ Δ heqM s S t t' T heqΓ heqt heqt' heqT hsS
+    cases heqM
+    cases heqΓ
+    cases heqt
+    cases heqt'
+    cases heqT
+    apply IsEqualTerm.sigma_first_eq
+    rotate_right
+    · apply B⌈1ₙ⇑ₛ(s/ₙhleq)⌉
+    · simp [lift_subst_n]
+      rw [←substitution_sigma]
+      apply ihppSi
+      repeat' rfl
+      apply hsS
+
+theorem substitution_gen_sigma_second_eq :
+    ∀ {n : Nat} {Γ : Ctx n} {p p' A : Tm n} {B : Tm (n + 1)},
+    (Γ ⊢ p ≡ p' ∶ ΣA;B) →
+    (∀ (m l : Nat) {leq : l ≤ m} (Γ_1 : Ctx l) (Δ : CtxGen (l + 1) (m + 1)) (eqM : n = m + 1) (s S : Tm l)
+        (a a' A_1 : Tm (m + 1 - 1 + 1)),
+        eqM ▸ Γ = Γ_1 ⬝ S ⊗ Δ →
+          eqM ▸ p = a →
+            eqM ▸ p' = a' →
+              (eqM ▸ ΣA;B) = A_1 →
+                (Γ_1 ⊢ s ∶ S) → Γ_1 ⊗ ⌈s⌉(Δ w/Nat.le_refl l) ⊢ a⌈s/ₙleq⌉ ≡ a'⌈s/ₙleq⌉ ∶ A_1⌈s/ₙleq⌉) →
+      ∀ (m l : Nat) {leq : l ≤ m} (Γ_1 : Ctx l) (Δ : CtxGen (l + 1) (m + 1)) (eqM : n = m + 1) (s S : Tm l)
+        (a a' A : Tm (m + 1 - 1 + 1)),
+        eqM ▸ Γ = Γ_1 ⬝ S ⊗ Δ →
+          eqM ▸ π₂ p = a →
+            eqM ▸ π₂ p' = a' →
+              eqM ▸ B⌈π₁ p⌉₀ = A → (Γ_1 ⊢ s ∶ S) → Γ_1 ⊗ ⌈s⌉(Δ w/Nat.le_refl l) ⊢ a⌈s/ₙleq⌉ ≡ a'⌈s/ₙleq⌉ ∶ A⌈s/ₙleq⌉ :=
+  by
+    intro n Γ' p p' A B hppSi ihppSi m l hleq Γ Δ heqM s S t t' T heqΓ heqt heqt' heqT hsS
     cases heqM
     cases heqΓ
     cases heqt
     cases heqt'
     cases heqT
     simp [substitution_zero_lift]
-    apply IsEqualTerm.sigma_elim_eq
-    · apply ihAA
-      · rfl
-      · rfl
-      · rfl
-      · apply hsS
-      · rfl
-    · simp [lift_subst_n]
-      rw [lift_n_substitution]
-      rw [extend_expand_context_n_substitution]
-      apply ihBB
-      · rfl
-      · rfl
-      · rfl
-      · apply hsS
-      · rfl
-    · simp [lift_subst_n]
-      rw [←substitution_sigma]
+    apply IsEqualTerm.sigma_second_eq
+    rotate_right
+    · apply A⌈(s/ₙhleq)⌉
+    · rw [←substitution_sigma]
       apply ihppSi
-      · rfl
-      · rfl
-      · rfl
-      · rfl
-      · apply hsS
-      · rfl
-    · simp [lift_subst_n]
-      rw [←substitution_sigma]
-      rw [lift_n_substitution]
-      rw [extend_expand_context_n_substitution]
-      apply ihCC
-      · rfl
-      · rfl
-      · rfl
-      · apply hsS
-      · rfl
-    · simp [lift_subst_n]
-      rw [subst_subst_sigma_C]
-      simp [lift_n_substitution]
-      rw [extend_expand_context_n_substitution]
-      rw [extend_expand_context_n_substitution]
-      apply ihccC
-      · rfl
-      · rfl
-      · rfl
-      · rfl
-      · apply hsS
-      · rfl
+      repeat' rfl
+      apply hsS
 
 theorem substitution_gen_iden_intro_eq : ∀ {n : Nat} {Γ : Ctx n} {A A' a a' : Tm n},
    Γ ⊢ A ≡ A' type →
