IMLTT/typed/proofs/admissable/WeakeningGeneral.lean
@@ -101,8 +101,10 @@ theorem weakening :
       apply weakening_empty_elim
     case HasTypePiElim =>
       apply weakening_pi_elim
-    case HasTypeSigmaElim =>
-      apply weakening_sigma_elim
+    case HasTypeSigmaFirst =>
+      apply weakening_sigma_first
+    case HasTypeSigmaSecond =>
+      apply weakening_sigma_second
     case HasTypeIdenElim =>
       apply weakening_iden_elim
     case HasTypeTyConv =>
@@ -133,8 +135,10 @@ theorem weakening :
       apply weakening_unit_comp
     case IsEqualTermPiComp =>
       apply weakening_pi_comp
-    case IsEqualTermSigmaComp =>
-      apply weakening_sigma_comp
+    case IsEqualTermSigmaFirstComp =>
+      apply weakening_sigma_first_comp
+    case IsEqualTermSigmaSecondComp =>
+      apply weakening_sigma_second_comp
     case IsEqualTermIdenComp =>
       apply weakening_iden_comp
     case IsEqualTermUnitIntroEq =>
@@ -149,8 +153,10 @@ theorem weakening :
       apply weakening_pi_elim_eq
     case IsEqualTermSigmaIntroEq =>
       apply weakening_sigma_intro_eq
-    case IsEqualTermSigmaElimEq =>
-      apply weakening_sigma_elim_eq
+    case IsEqualTermSigmaFirstEq =>
+      apply weakening_sigma_first_eq
+    case IsEqualTermSigmaSecondEq =>
+      apply weakening_sigma_second_eq
     case IsEqualTermIdenIntroEq =>
       apply weakening_iden_intro_eq
     case IsEqualTermIdenElimEq =>
