IMLTT/typed/proofs/boundary/HasType.lean
@@ -116,17 +116,21 @@ theorem boundary_pi_elim :
     · apply haA
     · apply And.right (pi_is_type_inversion ihfPi)
 
-theorem boundary_sigma_elim :
-    ∀ {n : Nat} {Γ : Ctx n} {A : Tm n} {B : Tm (n + 1)} {p : Tm n} {C : Tm (n + 1)} {c : Tm (n + 1 + 1)},
-    (Γ ⊢ p ∶ ΣA;B) →
-    (Γ ⬝ ΣA;B) ⊢ C type →
-    (Γ ⬝ A ⬝ B ⊢ c ∶ C⌈(ₛ↑ₚ↑ₚidₚ), v(1)&v(0)⌉) →
-    Γ ⊢ ΣA;B type → (Γ ⬝ ΣA;B) ⊢ C type → Γ ⬝ A ⬝ B ⊢ C⌈(ₛ↑ₚ↑ₚidₚ), v(1)&v(0)⌉ type → Γ ⊢ C⌈p⌉₀ type :=
+theorem boundary_sigma_first :
+    ∀ {n : Nat} {Γ : Ctx n} {p A : Tm n} {B : Tm (n + 1)}, (Γ ⊢ p ∶ ΣA;B) → Γ ⊢ ΣA;B type → Γ ⊢ A type :=
   by
-    intro n Γ A B p C c hpSi hC hcC ihpSi ihC ihcC
+    intro n Γ p A B hpSi ihpSi
+    have h := sigma_is_type_inversion ihpSi
+    apply And.left h
+
+theorem boundary_sigma_second :
+    ∀ {n : Nat} {Γ : Ctx n} {p A : Tm n} {B : Tm (n + 1)}, (Γ ⊢ p ∶ ΣA;B) → Γ ⊢ ΣA;B type → Γ ⊢ B⌈π₁ p⌉₀ type :=
+  by
+    intro n Γ p A B hpSi ihpSi
+    have h := sigma_is_type_inversion ihpSi
     apply substitution_type
-    · apply hpSi
-    · apply ihC
+    · apply HasType.sigma_first hpSi
+    · apply And.right h
 
 theorem boundary_iden_elim :
     ∀ {n : Nat} {Γ : Ctx n} {A : Tm n} {B : Tm (n + 1 + 1 + 1)} {b a a' p : Tm n},
