IMLTT/typed/proofs/boundary/IsEqualTerm.lean
@@ -75,37 +75,63 @@ theorem boundary_pi_comp :
       · apply haA
       · apply ihbB
 
-theorem boundary_sigma_comp :
-    ∀ {n : Nat} {Γ : Ctx n} {a A b : Tm n} {B C : Tm (n + 1)} {c : Tm (n + 1 + 1)},
-    (Γ ⊢ a ∶ A) → (Γ ⊢ b ∶ B⌈a⌉₀) → (Γ ⬝ ΣA;B) ⊢ C type →
-    (Γ ⬝ A ⬝ B ⊢ c ∶ C⌈(ₛ↑ₚ↑ₚidₚ), v(1)&v(0)⌉) →
-    Γ ⊢ A type → Γ ⊢ B⌈a⌉₀ type → (Γ ⬝ ΣA;B) ⊢ C type →
-    Γ ⬝ A ⬝ B ⊢ C⌈(ₛ↑ₚ↑ₚidₚ), v(1)&v(0)⌉ type →
-    (Γ ⊢ A.indSigma B C c (a&b) ∶ C⌈a&b⌉₀) ∧ (Γ ⊢ c⌈(ₛidₚ), a, b⌉ ∶ C⌈a&b⌉₀) ∧ Γ ⊢ C⌈a&b⌉₀ type :=
+theorem boundary_sigma_first_comp :
+    ∀ {n : Nat} {Γ : Ctx n} {a b A : Tm n} {B : Tm (n + 1)},
+  (Γ ⊢ a ∶ A) →
+    (Γ ⊢ b ∶ B⌈a⌉₀) →
+      Γ ⊢ ΣA;B type → Γ ⊢ A type → Γ ⊢ B⌈a⌉₀ type → Γ ⊢ ΣA;B type → (Γ ⊢ π₁ a&b ∶ A) ∧ (Γ ⊢ a ∶ A) ∧ Γ ⊢ A type :=
   by
-    intro n Γ a A b B C c haA hbB hC hcC ihaA ihbB ihC ihcC
+    intro n Γ a b A B haA hbB hSi ihaA ihbB ihSi
     repeat' apply And.intro
-    · apply HasType.sigma_elim
-      · apply HasType.sigma_intro
-        · apply haA
-        · apply hbB
-        · apply ctx_extr (boundary_ctx_term hcC)
-      · apply hC
-      · apply hcC
-    · rw [←boundary_helper_sigma_elim]
-      simp [substitution_twice_zero]
-      apply substitution_term
+    · apply HasType.sigma_first
+      apply HasType.sigma_intro
       · apply haA
-      · apply substitution_term
-        rotate_left
-        · apply hcC
-        · sorry -- XXX: might be trouble
-    · apply substitution_type
-      · apply HasType.sigma_intro
+      · apply hbB
+      · have h := sigma_is_type_inversion hSi
+        apply And.right h
+    · apply haA
+    · apply ihaA
+
+theorem boundary_sigma_second_comp :
+    ∀ {n : Nat} {Γ : Ctx n} {a b A : Tm n} {B : Tm (n + 1)},
+  (Γ ⊢ a ∶ A) →
+    (Γ ⊢ b ∶ B⌈a⌉₀) →
+      Γ ⊢ ΣA;B type →
+        Γ ⊢ A type →
+          Γ ⊢ B⌈a⌉₀ type → Γ ⊢ ΣA;B type → (Γ ⊢ π₂ a&b ∶ B⌈π₁ a&b⌉₀) ∧ (Γ ⊢ b ∶ B⌈π₁ a&b⌉₀) ∧ Γ ⊢ B⌈π₁ a&b⌉₀ type :=
+  by
+    intro n Γ a b A B haA hbB hSi ihaA ihbB ihSi
+    repeat' apply And.intro
+    · apply HasType.sigma_second
+      apply HasType.sigma_intro
+      · apply haA
+      · apply hbB
+      · have h := sigma_is_type_inversion hSi
+        apply And.right h
+    · apply HasType.ty_conv
+      · apply hbB
+      · have h := sigma_is_type_inversion hSi
+        apply functionality_typing_type
+        · apply And.right h
+        · apply IsEqualTerm.term_symm
+          apply IsEqualTerm.sigma_first_comp
+          · apply haA
+          · apply hbB
+          · apply hSi
+        · apply haA
+        · apply HasType.sigma_first
+          apply HasType.sigma_intro
+          · apply haA
+          · apply hbB
+          · apply And.right h
+    · have h := sigma_is_type_inversion hSi
+      apply substitution_type
+      · apply HasType.sigma_first
+        apply HasType.sigma_intro
         · apply haA
         · apply hbB
-        · apply ctx_extr (boundary_ctx_term hcC)
-      · apply hC
+        · apply And.right h
+      · apply And.right h
 
 theorem boundary_iden_comp :
     ∀ {n : Nat} {Γ : Ctx n} {A : Tm n} {B : Tm (n + 1 + 1 + 1)} {b a : Tm n},
@@ -302,71 +328,47 @@ theorem boundary_sigma_intro_eq :
       · apply And.right (And.right ihaaA)
       · apply hB
 
-theorem boundary_sigma_elim_eq :
-    ∀ {n : Nat} {Γ : Ctx n} {A : Tm n} {B : Tm (n + 1)} {A' : Tm n} {B' : Tm (n + 1)} {p p' : Tm n} {C C' : Tm (n + 1)}
-  {c c' : Tm (n + 1 + 1)},
-  Γ ⊢ A ≡ A' type →
-    Γ ⬝ A ⊢ B ≡ B' type →
-      (Γ ⊢ p ≡ p' ∶ ΣA;B) →
-        (Γ ⬝ ΣA;B) ⊢ C ≡ C' type →
-          (Γ ⬝ A ⬝ B ⊢ c ≡ c' ∶ C⌈(ₛ↑ₚ↑ₚidₚ), v(1)&v(0)⌉) →
-            Γ ⊢ A type ∧ Γ ⊢ A' type →
-              Γ ⬝ A ⊢ B type ∧ Γ ⬝ A ⊢ B' type →
-                (Γ ⊢ p ∶ ΣA;B) ∧ (Γ ⊢ p' ∶ ΣA;B) ∧ Γ ⊢ ΣA;B type →
-                  (Γ ⬝ ΣA;B) ⊢ C type ∧ (Γ ⬝ ΣA;B) ⊢ C' type →
-                    (Γ ⬝ A ⬝ B ⊢ c ∶ C⌈(ₛ↑ₚ↑ₚidₚ), v(1)&v(0)⌉) ∧
-                        (Γ ⬝ A ⬝ B ⊢ c' ∶ C⌈(ₛ↑ₚ↑ₚidₚ), v(1)&v(0)⌉) ∧ Γ ⬝ A ⬝ B ⊢ C⌈(ₛ↑ₚ↑ₚidₚ), v(1)&v(0)⌉ type →
-                      (Γ ⊢ A.indSigma B C c p ∶ C⌈p⌉₀) ∧ (Γ ⊢ A'.indSigma B' C' c' p' ∶ C⌈p⌉₀) ∧ Γ ⊢ C⌈p⌉₀ type :=
+theorem boundary_sigma_first_eq :
+    ∀ {n : Nat} {Γ : Ctx n} {p p' A : Tm n} {B : Tm (n + 1)},
+    (Γ ⊢ p ≡ p' ∶ ΣA;B) → (Γ ⊢ p ∶ ΣA;B) ∧ (Γ ⊢ p' ∶ ΣA;B) ∧ Γ ⊢ ΣA;B type → (Γ ⊢ π₁ p ∶ A) ∧ (Γ ⊢ π₁ p' ∶ A) ∧ Γ ⊢ A type :=
   by
-    intro n Γ A B A' B' p p' C C' c c' hAA hBB hppSi hCC hccC ihAA ihBB ihppSi ihCC ihccC
+    intro n Γ p p' A B hppSi ihppSi
     repeat' apply And.intro
-    · apply HasType.sigma_elim
-      · apply And.left ihppSi
-      · apply And.left ihCC
-      · apply And.left ihccC
+    · apply HasType.sigma_first
+      apply And.left ihppSi
+    · apply HasType.sigma_first
+      apply And.left (And.right ihppSi)
+    · have h := sigma_is_type_inversion (And.right (And.right ihppSi))
+      apply And.left h
+
+theorem boundary_sigma_second_eq :
+    ∀ {n : Nat} {Γ : Ctx n} {p p' A : Tm n} {B : Tm (n + 1)},
+    (Γ ⊢ p ≡ p' ∶ ΣA;B) →
+    (Γ ⊢ p ∶ ΣA;B) ∧ (Γ ⊢ p' ∶ ΣA;B) ∧ Γ ⊢ ΣA;B type →
+      (Γ ⊢ π₂ p ∶ B⌈π₁ p⌉₀) ∧ (Γ ⊢ π₂ p' ∶ B⌈π₁ p⌉₀) ∧ Γ ⊢ B⌈π₁ p⌉₀ type :=
+  by
+    intro n Γ p p' A B hppSi ihppSi
+    repeat' apply And.intro
+    · apply HasType.sigma_second
+      apply And.left ihppSi
     · apply HasType.ty_conv
-      · apply HasType.sigma_elim
-        · apply HasType.ty_conv
-          · apply And.left (And.right ihppSi)
-          · apply IsEqualType.sigma_form_eq hAA hBB
-        · apply context_conversion_type
-          · apply IsType.sigma_form
-            · apply And.right ihAA
-            · apply context_conversion_type
-              · apply And.right ihAA
-              · apply hAA
-              · apply And.right ihBB
-          · apply IsEqualType.sigma_form_eq hAA hBB
-          · apply And.right ihCC
-        · rw [←empty_expand_context (Γ := Γ)]
-          rw [extend_expand_context]
-          rw [extend_expand_context]
-          rw [middle_expand_context]
-          apply And.left (And.right (And.right context_conversion))
-          rotate_left
-          · apply hAA
-          · apply And.left ihAA
-          · apply And.right ihAA
-          · simp [expand_ctx]
-            apply context_conversion_term
-            · apply And.right ihBB
-            · apply hBB
-            · apply HasType.ty_conv
-              · apply And.left (And.right ihccC)
-              · sorry
-      · apply IsEqualType.type_symm
-        apply IsEqualType.type_trans
-        · apply functionality_typing_type
-          · apply And.left ihCC
-          · apply hppSi
-          · apply And.left ihppSi
-          · apply And.left (And.right ihppSi)
-        · apply substitution_type_eq
-          · apply And.left (And.right ihppSi)
-          · apply hCC
-    · apply substitution_type
-      · apply And.left ihppSi
-      · apply And.left ihCC
+      · apply HasType.sigma_second
+        apply And.left (And.right ihppSi)
+      · have h := sigma_is_type_inversion (And.right (And.right ihppSi))
+        apply functionality_typing_type
+        · apply And.right h
+        · apply IsEqualTerm.term_symm
+          apply IsEqualTerm.sigma_first_eq
+          apply hppSi
+        · apply HasType.sigma_first
+          apply And.left (And.right ihppSi)
+        · apply HasType.sigma_first
+          apply And.left ihppSi
+    · have h := sigma_is_type_inversion (And.right (And.right ihppSi))
+      apply substitution_type
+      · apply HasType.sigma_first
+        apply And.left ihppSi
+      · apply And.right h
 
 theorem boundary_iden_intro_eq :
     ∀ {n : Nat} {Γ : Ctx n} {A A' a a' : Tm n},
