IMLTT/untyped/proofs/Composition.lean
@@ -97,17 +97,12 @@ theorem weakening_comp {ρ : Weak l m} {ρ' : Weak m n} {t : Tm n} :
       apply And.intro
       · apply weakening_comp
       · apply weakening_comp
-    | .indSigma A B C c p =>
+    | .firstSigma p =>
       simp [weaken]
-      apply And.intro
-      · apply weakening_comp
-      · apply And.intro
-        · apply weakening_comp
-        · apply And.intro
-          · apply weakening_comp
-          · apply And.intro
-            · apply weakening_comp
-            · apply weakening_comp
+      apply weakening_comp
+    | .secondSigma p =>
+      simp [weaken]
+      apply weakening_comp
     | .refl A a =>
       simp [weaken]
       apply And.intro
@@ -526,25 +521,14 @@ theorem substitution_comp_ρσ {t : Tm n} :
       apply And.intro
       · apply substitution_comp_ρσ
       · apply substitution_comp_ρσ
-    | .indSigma A B C c p =>
+    | .firstSigma p =>
       simp [substitute]
       simp [weaken]
-      apply And.intro
-      · apply substitution_comp_ρσ
-      · apply And.intro
-        · simp [lift_weak_n]
-          simp [lift_subst_n]
-          rw [←substitution_lift_comp_ρσ]
-          apply substitution_comp_ρσ
-        · apply And.intro
-          · simp [lift_weak_n]
-            simp [lift_subst_n]
-            rw [←substitution_lift_comp_ρσ]
-            apply substitution_comp_ρσ
-          · apply And.intro
-            · rw [←substitution_lift_n_comp_ρσ]
-              apply substitution_comp_ρσ
-            · apply substitution_comp_ρσ
+      apply substitution_comp_ρσ
+    | .secondSigma p =>
+      simp [substitute]
+      simp [weaken]
+      apply substitution_comp_ρσ
     | .refl A a =>
       simp [substitute]
       simp [weaken]
@@ -815,26 +799,14 @@ theorem substitution_comp_σρ {t : Tm n} :
       apply And.intro
       · apply substitution_comp_σρ
       · apply substitution_comp_σρ
-    | .indSigma A B C c p =>
+    | .firstSigma p =>
       simp [weaken]
       simp [substitute]
-      apply And.intro
-      · apply substitution_comp_σρ
-      · apply And.intro
-        · simp [lift_weak_n]
-          simp [lift_subst_n]
-          rw [←substitution_lift_comp_σρ]
-          apply substitution_comp_σρ
-        · apply And.intro
-          · simp [lift_weak_n]
-            simp [lift_subst_n]
-            rw [←substitution_lift_comp_σρ]
-            apply substitution_comp_σρ
-          · apply And.intro
-            · simp [lift_weak_n]
-              rw [←substitution_lift_n_comp_σρ]
-              apply substitution_comp_σρ
-            · apply substitution_comp_σρ
+      apply substitution_comp_σρ
+    | .secondSigma p =>
+      simp [weaken]
+      simp [substitute]
+      apply substitution_comp_σρ
     | .refl A a =>
       simp [weaken]
       simp [substitute]
@@ -1085,22 +1057,12 @@ theorem substitution_comp :
       apply And.intro
       · apply substitution_comp
       · apply substitution_comp
-    | indSigma A B C c p =>
+    | firstSigma p =>
       simp [substitute]
-      apply And.intro
-      · apply substitution_comp
-      · apply And.intro
-        · simp [lift_subst_n]
-          rw [←substitution_lift_comp]
-          apply substitution_comp
-        · apply And.intro
-          · simp [lift_subst_n]
-            rw [←substitution_lift_comp]
-            apply substitution_comp
-          · apply And.intro
-            · rw [←substitution_lift_n_comp]
-              apply substitution_comp
-            · apply substitution_comp
+      apply substitution_comp
+    | secondSigma p =>
+      simp [substitute]
+      apply substitution_comp
     | refl A a =>
       simp [substitute]
       apply And.intro
