IMLTT/untyped/proofs/Conversion.lean
@@ -150,29 +150,16 @@ theorem conversion_var_substitute {σ σ' : Subst m n} :
         assumption
       · apply conversion_var_substitute h
         assumption
-    | .indSigma A B C c p =>
+    | .firstSigma p =>
       simp [substitute]
       simp [weaken]
-      apply And.intro
-      · apply conversion_var_substitute h
-        assumption
-      · apply And.intro
-        · apply conversion_var_substitute
-          · have ξ := lift_subst_n 1 σ
-            apply ξ
-          · apply conversion_var_lift_n h
-        · apply And.intro
-          · apply conversion_var_substitute
-            · have ξ := lift_subst_n 1 σ
-              apply ξ
-            · apply conversion_var_lift_n h
-          · apply And.intro
-            · apply conversion_var_substitute
-              · have ξ := lift_subst_n 2 σ
-                apply ξ
-              · apply conversion_var_lift_n h
-            · apply conversion_var_substitute h
-              assumption
+      apply conversion_var_substitute h
+      assumption
+    | .secondSigma p =>
+      simp [substitute]
+      simp [weaken]
+      apply conversion_var_substitute h
+      assumption
     | .refl A a =>
       simp [substitute]
       simp [weaken]
@@ -295,27 +282,14 @@ theorem conversion_sub_weak :
       apply And.intro
       · apply conversion_sub_weak
       · apply conversion_sub_weak
-    | indSigma A B C c p =>
+    | firstSigma p =>
       simp [substitute]
       simp [weaken]
-      apply And.intro
-      · apply conversion_sub_weak
-      · apply And.intro
-        · apply conversion_var_substitute
-          · apply lift_subst_n 1 (.weak ρ)
-          · apply conversion_var_lift_n
-            apply conversion_var_sub_weak
-        · apply And.intro
-          · apply conversion_var_substitute
-            · apply lift_subst_n 1 (.weak ρ)
-            · apply conversion_var_lift_n
-              apply conversion_var_sub_weak
-          · apply And.intro
-            · apply conversion_var_substitute
-              · apply lift_subst_n 2 (.weak ρ)
-              · apply conversion_var_lift_n
-                apply conversion_var_sub_weak
-            · apply conversion_sub_weak
+      apply conversion_sub_weak
+    | secondSigma p =>
+      simp [substitute]
+      simp [weaken]
+      apply conversion_sub_weak
     | refl A a =>
       simp [substitute]
       simp [weaken]
